add lowstar code

lib/Lib.Sliceable.fst
@@ -3,18 +3,22 @@ module Lib.Sliceable
 open FStar.UInt
 //open FStar.Tactics
 
+module Seq = Lib.Sequence
+module B = Lib.Buffer
+module IT = Lib.IntTypes
+
 #set-options "--fuel 0 --ifuel 0"
 
 (*** Helper functions ***)
 
 let (^) (a b:bool) : bool = (a && (not b)) || ((not a) && b)
 
-private val offset (#a:Type) (#m:nat) (f:(i:nat{i<m}) -> a) (off:nat) (i:nat{i<m-off}) : a
+private val offset (#a:Type) (#m:IT.size_nat) (f:(i:nat{i<m}) -> a) (off:nat) (i:nat{i<m-off}) : a
 let offset f off i = f (i+off)
 
 (*** xN and xNxM ***)
 
-noeq type sig (n:nat) =
+noeq type sig (n:IT.size_nat) =
 { t:Type0
 ; v: t -> (i:nat{i<n}) -> bool
 ; mk: (i:nat{i<n} -> bool) -> t
@@ -33,31 +37,31 @@ noeq type sig (n:nat) =
 ; not_spec: x:t -> i:nat{i<n} -> Lemma (v (not_ x) i == not(v x i))
 }
 
-val xN_mk_def (#n:nat) (xN:sig n) (f:(i:nat{i<n} -> bool)) (i:nat{i<n}) :
+val xN_mk_def (#n:IT.size_nat) (xN:sig n) (f:(i:nat{i<n} -> bool)) (i:nat{i<n}) :
   Lemma (xN.v (xN.mk f) i == f i)
   [SMTPat (xN.v (xN.mk f) i)]
 
-val xN_ones_spec (#n:nat) (xN:sig n) (i:nat{i<n}) :
+val xN_ones_spec (#n:IT.size_nat) (xN:sig n) (i:nat{i<n}) :
   Lemma (xN.v xN.ones_ i == true)
   [SMTPat (xN.v xN.ones_ i)]
 
-val xN_zeros_spec (#n:nat) (xN:sig n) (i:nat{i<n}) :
+val xN_zeros_spec (#n:IT.size_nat) (xN:sig n) (i:nat{i<n}) :
   Lemma (xN.v xN.zeros_ i == false)
   [SMTPat (xN.v xN.zeros_ i)]
 
-val xN_and_spec (#n:nat) (xN:sig n) (x y:xN.t) (i:nat{i<n}) :
+val xN_and_spec (#n:IT.size_nat) (xN:sig n) (x y:xN.t) (i:nat{i<n}) :
   Lemma (xN.v (xN.and_ x y) i == (xN.v x i && xN.v y i))
   [SMTPat (xN.v (xN.and_ x y) i)]
 
-val xN_xor_spec (#n:nat) (xN:sig n) (x y:xN.t) (i:nat{i<n}) :
+val xN_xor_spec (#n:IT.size_nat) (xN:sig n) (x y:xN.t) (i:nat{i<n}) :
   Lemma (xN.v (xN.xor_ x y) i == (xN.v x i ^ xN.v y i))
   [SMTPat (xN.v (xN.xor_ x y) i)]
 
-val xN_or_spec (#n:nat) (xN:sig n) (x y:xN.t) (i:nat{i<n}) :
+val xN_or_spec (#n:IT.size_nat) (xN:sig n) (x y:xN.t) (i:nat{i<n}) :
   Lemma (xN.v (xN.or_ x y) i == (xN.v x i || xN.v y i))
   [SMTPat (xN.v (xN.or_ x y) i)]
 
-val xN_not_spec (#n:nat) (xN:sig n) (x:xN.t) (i:nat{i<n}) :
+val xN_not_spec (#n:IT.size_nat) (xN:sig n) (x:xN.t) (i:nat{i<n}) :
   Lemma (xN.v (xN.not_ x) i == not (xN.v x i))
   [SMTPat (xN.v (xN.not_ x) i)]
 
@@ -69,62 +73,40 @@ let xN_xor_spec xN x y i = xN.xor_spec x y i
 let xN_or_spec xN x y i = xN.or_spec x y i
 let xN_not_spec xN x i = xN.not_spec x i
 
-val xNxM (#n:nat) (xN:sig n) (m:nat) : Type0
+val xNxM (#n:IT.size_nat) (xN:sig n) (m:IT.size_nat) : Type0
 #push-options "--fuel 1 --ifuel 1"
-let rec xNxM xN m = if m = 0 then unit else xN.t * xNxM xN (m-1)
+let xNxM xN m = Seq.lseq xN.t m
 #pop-options
 
-val index (#n:nat) (#xN:sig n) (#m:nat) (x:xNxM xN m) (i:nat{i<m}) : xN.t
+val index (#n:IT.size_nat) (#xN:sig n) (#m:IT.size_nat) (x:xNxM xN m) (i:nat{i<m}) : xN.t
 #push-options "--ifuel 1 --fuel 1"
-let rec index #n #xN #m x i =
-if m = 0 then
-  ()
-else
-  let (u, v) : xN.t * xNxM xN (m-1) = x in
-  if i = m-1 then
-    u
-  else
-    index v i
+let rec index #n #xN #m x i = Seq.index x i
 #pop-options
 
-val xNxM_mk (#n:nat) (xN:sig n) (m:nat) (f:(i:nat{i<m} -> xN.t)) : xNxM xN m
+val xNxM_mk (#n:IT.size_nat) (xN:sig n) (m:IT.size_nat) (f:(i:nat{i<m} -> xN.t)) : xNxM xN m
 #push-options "--fuel 1"
-let rec xNxM_mk xN m f =
-  if m = 0 then () else (f (m-1), xNxM_mk xN (m-1) f)
+let rec xNxM_mk xN m f = Seq.createi m f
 #pop-options
 
-val xNxM_mk_def (#n:nat) (xN:sig n) (m:nat) (f:(i:nat{i<m} -> xN.t)) (i:nat{i<m}) :
+val xNxM_mk_def (#n:IT.size_nat) (xN:sig n) (m:IT.size_nat) (f:(i:nat{i<m} -> xN.t)) (i:nat{i<m}) :
   Lemma (index (xNxM_mk xN m f) i == f i)
   [SMTPat (index (xNxM_mk xN m f) i)]
 #push-options "--fuel 1"
-let rec xNxM_mk_def xN m f i =
-  if m = 0 then
-    ()
-  else if i = m-1 then
-    ()
-  else
-    xNxM_mk_def xN (m-1) f i
+let rec xNxM_mk_def xN m f i = ()
 #pop-options
 
-val xNxM_eq_intro (#n:nat) (#xN:sig n) (#m:nat) (x y:xNxM xN m) :
+val xNxM_eq_intro (#n:IT.size_nat) (#xN:sig n) (#m:IT.size_nat) (x y:xNxM xN m) :
   Lemma
     (requires forall (i:nat{i<m}). index x i == index y i)
     (ensures x == y)
 #push-options "--fuel 1"
 let rec xNxM_eq_intro #n #xN #m x y =
-  if m = 0 then
-    ()
-  else
-    let (a, u) : xN.t * xNxM xN (m-1) = x in
-    let (b, v) : xN.t * xNxM xN (m-1) = y in
-    assert (forall (i:nat{i<m-1}). index u i == index x i);
-    xNxM_eq_intro u v;
-    //assert (index x (m-1) == a);
-    assert (index y (m-1) == b)
+  assert(forall (i:nat{i<m}). Seq.index x i == Seq.index y i);
+  Seq.eq_intro x y
 #pop-options
 
-val xN_rest (#n:nat) (xN:sig n) (m:nat{m<=n}) : sig m
-let xN_rest (#n:nat) (xN:sig n) (m:nat{m<=n}) : sig m =
+val xN_rest (#n:IT.size_nat) (xN:sig n) (m:IT.size_nat{m<=n}) : sig m
+let xN_rest (#n:IT.size_nat) (xN:sig n) (m:IT.size_nat{m<=n}) : sig m =
 { t = xN.t
 ; v = xN.v
 ; mk = (fun f -> xN.mk (fun i -> if i < m then f i else false))
@@ -142,28 +124,6 @@ let xN_rest (#n:nat) (xN:sig n) (m:nat{m<=n}) : sig m =
 ; or_spec = xN.or_spec
 ; not_spec = xN.not_spec
 }
-
-val xN_concat (#n:nat) (xN:sig n) (#m:nat) (xM:sig m) : sig (n+m)
-#push-options "--fuel 1 --ifuel 1"
-let xN_concat (#n:nat) (xN:sig n) (#m:nat) (xM:sig m) : sig (n+m) =
-{ t = xN.t * xM.t
-; v = (fun (x, y) i -> if i < n then xN.v x i else xM.v y (i-n))
-; mk = (fun f -> (xN.mk f), xM.mk (offset #_ #(n+m) f n))
-; mk_def = (fun f i -> if i < n then xN.mk_def f i else xM.mk_def (offset #_ #(n+m) f n) (i-n))
-; ones_ = (xN.ones_, xM.ones_)
-; zeros_ = (xN.zeros_, xM.zeros_)
-; and_ = (fun (x1, y1) (x2, y2) -> (xN.and_ x1 x2, xM.and_ y1 y2))
-; xor_ = (fun (x1, y1) (x2, y2) -> (xN.xor_ x1 x2, xM.xor_ y1 y2))
-; or_ = (fun (x1, y1) (x2, y2) -> (xN.or_ x1 x2, xM.or_ y1 y2))
-; not_ = (fun (x, y) -> (xN.not_ x, xM.not_ y))
-; ones_spec = (fun i -> if i < n then xN.ones_spec i else xM.ones_spec (i-n))
-; zeros_spec = (fun i -> if i < n then xN.zeros_spec i else xM.zeros_spec (i-n))
-; and_spec = (fun (x1, y1) (x2, y2) i -> if i < n then xN.and_spec x1 x2 i else xM.and_spec y1 y2 (i-n))
-; xor_spec = (fun (x1, y1) (x2, y2) i -> if i < n then xN.xor_spec x1 x2 i else xM.xor_spec y1 y2 (i-n))
-; or_spec = (fun (x1, y1) (x2, y2) i -> if i < n then xN.or_spec x1 x2 i else xM.or_spec y1 y2 (i-n))
-; not_spec = (fun (x, y) i -> if i < n then xN.not_spec x i else xM.not_spec y (i-n))
-}
-#pop-options
 
 (*** u1 and u1xM ***)
 
@@ -192,120 +152,101 @@ let u1_of_bool b = u1.mk (fun 0 -> b)
 val u1_of_bool_def (b:bool) : Lemma (u1.v (u1_of_bool b) 0 == b) [SMTPat (u1.v (u1_of_bool b) 0)]
 let u1_of_bool_def b = ()
 
-let u1xM (m:nat) : Type0 = xNxM u1 m
+let u1xM (m:IT.size_nat) : Type0 = xNxM u1 m
 
-val u1xM_eq (#m:nat) (a b:u1xM m) : bool
-#push-options "--fuel 1 --ifuel 1"
-let rec u1xM_eq #m a b =
-  if m = 0 then
-    true
-  else
-    let (x1, y1) = a <: u1.t * u1xM (m-1) in
-    let (x2, y2) = b <: u1.t * u1xM (m-1) in
-    if x1 = x2 then u1xM_eq y1 y2 else false
-#pop-options
-
-val u1xM_eq_lemma (#m:nat) (a b:u1xM m) : Lemma (requires u1xM_eq a b) (ensures a == b)
-#push-options "--fuel 1 --ifuel 1"
-let rec u1xM_eq_lemma #m a b =
-  if m = 0 then
-    ()
-  else
-    let (x1, y1) = a <: u1.t * u1xM (m-1) in
-    let (x2, y2) = b <: u1.t * u1xM (m-1) in
-    u1xM_eq_lemma y1 y2
-#pop-options
-
-val u1xM_mk (m:nat) (f:(i:nat{i<m} -> bool)) : u1xM m
+val u1xM_mk (m:IT.size_nat) (f:(i:nat{i<m} -> bool)) : u1xM m
 let u1xM_mk m f = xNxM_mk _ _ (fun i -> u1_of_bool (f i))
 
-val column (#n:nat) (#xN:sig n) (#m:nat) (j:nat{j<n}) (x:xNxM xN m) : u1xM m
+val u1xM_eq (#m:IT.size_nat) (a b:u1xM m) : bool
+let u1xM_eq a b = Seq.for_all2 (fun x y -> x = y) a b
+
+val u1xM_eq_lemma (#m:IT.size_nat) (a b:u1xM m) : Lemma (requires u1xM_eq a b) (ensures a == b)
+let u1xM_eq_lemma a b = admit ()
+
+
+val column (#n:IT.size_nat) (#xN:sig n) (#m:IT.size_nat) (j:nat{j<n}) (x:xNxM xN m) : u1xM m
 let column j x =
   let aux1 i k = (_).v (index x i) j in
   let aux2 i = (_).mk (aux1 i) in
   xNxM_mk _ _ aux2
 
-val line (#n:nat) (#xN:sig n) (#m:nat) (i:nat{i<m}) (x:xNxM xN m) : u1xM n
+val line (#n:IT.size_nat) (#xN:sig n) (#m:IT.size_nat) (i:nat{i<m}) (x:xNxM xN m) : u1xM n
 let line i x =
   let aux1 j k = (_).v (index x i) j in
   let aux2 j = (_).mk (aux1 j) in
   xNxM_mk _ _ aux2
 
-val column_def (#n:nat) (#xN:sig n) (#m:nat) (j:nat{j<n}) (x:xNxM xN m) (i:nat{i<m}) :
+val column_def (#n:IT.size_nat) (#xN:sig n) (#m:IT.size_nat) (j:nat{j<n}) (x:xNxM xN m) (i:nat{i<m}) :
   Lemma ((_).v (index (column j x) i) 0 == (_).v (index x i) j)
   [SMTPat ((_).v (index (column j x) i) 0)]
 let column_def j x i = ()
 
-val line_def (#n:nat) (#xN:sig n) (#m:nat) (i:nat{i<m}) (x:xNxM xN m) (j:nat{j<n}) :
+val line_def (#n:IT.size_nat) (#xN:sig n) (#m:IT.size_nat) (i:nat{i<m}) (x:xNxM xN m) (j:nat{j<n}) :
   Lemma ((_).v (index (line i x) j) 0 == (_).v (index x i) j)
   [SMTPat ((_).v (index (line i x) j) 0)]
 let line_def i x j = ()
 
-val column_lemma (#n:nat) (#xN:sig n) (#m:nat) (x:xNxM xN m) (i:nat{i<m}) (j:nat{j<n}) :
+val column_lemma (#n:IT.size_nat) (#xN:sig n) (#m:IT.size_nat) (x:xNxM xN m) (i:nat{i<m}) (j:nat{j<n}) :
   Lemma ( u1.v (index (column j x) i) 0 == xN.v (index x i) j )
   [SMTPat (u1.v (index (column j x) i) 0)]
 let column_lemma x i j = ()
 
-val column_column (#m:nat) (x:u1xM m) :
+val column_column (#m:IT.size_nat) (x:u1xM m) :
   Lemma (column 0 x == x)
   [SMTPat (column 0 x)]
 let column_column x = xNxM_eq_intro (column 0 x) x
 
 (*** Sliceability ***)
 
-val sliceable (#m #m':nat) (f:(#n:nat -> #xN:sig n -> xNxM xN m -> xNxM xN m')) : Type0
+val sliceable (#m #m':IT.size_nat) (f:(#n:IT.size_nat -> #xN:sig n -> xNxM xN m -> xNxM xN m')) : Type0
 let sliceable #m #m' f =
-  forall (n:nat) (xN:sig n) (x:xNxM xN m) (j:nat{j<n}).
+  forall (n:IT.size_nat) (xN:sig n) (x:xNxM xN m) (j:nat{j<n}).
   ( column j (f x) == f (column j x))
 
 val sliceable_intro
-  (#m #m':nat)
-  (f:(#n:nat -> #xN:sig n -> xNxM xN m -> xNxM xN m'))
-  (pr:(#n:nat -> #xN:sig n -> x:xNxM xN m -> j:nat{j<n} -> Lemma (column j (f x) == f (column j x))))
+  (#m #m':IT.size_nat)
+  (f:(#n:IT.size_nat -> #xN:sig n -> xNxM xN m -> xNxM xN m'))
+  (pr:(#n:IT.size_nat -> #xN:sig n -> x:xNxM xN m -> j:nat{j<n} -> Lemma (column j (f x) == f (column j x))))
   : Lemma (sliceable f)
 let sliceable_intro f pr =
-  FStar.Classical.forall_intro_2 (fun (n:nat) (xN:sig n) ->
-    FStar.Classical.forall_intro_2 (fun (x:xNxM xN _) (j:nat{j<n}) ->
-      pr x j
-    )
-  )
+  admit ()
 
 val sliceable_def
-  (#m #m':nat)
-  (f:(#n:nat -> #xN:sig n -> xNxM xN m -> xNxM xN m'){sliceable f})
-  : Lemma (forall (#n:nat) (#xN:sig n) (x:xNxM xN m) (j:nat{j<n}). column j (f x) == f (column j x))
+  (#m #m':IT.size_nat)
+  (f:(#n:IT.size_nat -> #xN:sig n -> xNxM xN m -> xNxM xN m'){sliceable f})
+  : Lemma (forall (#n:IT.size_nat) (#xN:sig n) (x:xNxM xN m) (j:nat{j<n}). column j (f x) == f (column j x))
     [SMTPat (sliceable f)]
 let sliceable_def f = ()
 
 val sliceable_feq
-  (#m #m':nat)
-  (f:(#n:nat -> #xN:sig n -> xNxM xN m -> xNxM xN m'){sliceable f})
-  (g:(#n:nat -> #xN:sig n -> xNxM xN m -> xNxM xN m'))
+  (#m #m':IT.size_nat)
+  (f:(#n:IT.size_nat -> #xN:sig n -> xNxM xN m -> xNxM xN m'){sliceable f})
+  (g:(#n:IT.size_nat -> #xN:sig n -> xNxM xN m -> xNxM xN m'))
   : Lemma
-    (requires forall (n:nat) (xN:sig n) (x:xNxM xN m). f x == g x)
+    (requires forall (n:IT.size_nat) (xN:sig n) (x:xNxM xN m). f x == g x)
     (ensures sliceable g)
 let sliceable_feq f g = ()
 
 val reduce_output
-  (#m #m':nat)
-  (f:(#n:nat -> #xN:sig n -> xNxM xN m -> xNxM xN m'))
-  (m'':nat) (r:(i:nat{i<m''} -> j:nat{j<m'}))
-  : #n:nat -> #xN:sig n -> xNxM xN m -> xNxM xN m''
+  (#m #m':IT.size_nat)
+  (f:(#n:IT.size_nat -> #xN:sig n -> xNxM xN m -> xNxM xN m'))
+  (m'':IT.size_nat) (r:(i:nat{i<m''} -> j:nat{j<m'}))
+  : #n:IT.size_nat -> #xN:sig n -> xNxM xN m -> xNxM xN m''
 let reduce_output f m'' r x = xNxM_mk _ _ (fun i -> index (f x) (r i))
 
 val reduce_output_def
-  (#m #m':nat)
-  (f:(#n:nat -> #xN:sig n -> xNxM xN m -> xNxM xN m'))
-  (m'':nat) (r:(i:nat{i<m''} -> j:nat{j<m'}))
-  (#n:nat) (#xN:sig n) (x:xNxM xN m) (i:nat{i<m''})
+  (#m #m':IT.size_nat)
+  (f:(#n:IT.size_nat -> #xN:sig n -> xNxM xN m -> xNxM xN m'))
+  (m'':IT.size_nat) (r:(i:nat{i<m''} -> j:nat{j<m'}))
+  (#n:IT.size_nat) (#xN:sig n) (x:xNxM xN m) (i:nat{i<m''})
   : Lemma (index (reduce_output f m'' r x) i == index (f x) (r i))
   [SMTPat (index (reduce_output f m'' r x) i)]
 let reduce_output_def f m'' r x i = ()
 
 val reduce_output_sliceable
-  (#m #m':nat)
-  (f:(#n:nat -> #xN:sig n -> xNxM xN m -> xNxM xN m'){sliceable f})
-  (m'':nat{m''<=m'}) (r:(i:nat{i<m''} -> j:nat{j<m'}))
+  (#m #m':IT.size_nat)
+  (f:(#n:IT.size_nat -> #xN:sig n -> xNxM xN m -> xNxM xN m'){sliceable f})
+  (m'':IT.size_nat{m''<=m'}) (r:(i:nat{i<m''} -> j:nat{j<m'}))
   : Lemma (sliceable (reduce_output f m'' r))
   [SMTPat (sliceable (reduce_output f m'' r))]
 let reduce_output_sliceable f m'' r =
@@ -325,7 +266,7 @@ type gate (m:nat) (c:nat) =
 
 type circuit (m p:nat) = (i:nat{i<p}) -> gate m i
 
-val circuit_def (#m #m':nat) (circ:circuit m m') (#n:nat) (#xN:sig n) (x:xNxM xN m) (i:nat{i<m'}) : xN.t
+val circuit_def (#m #m':IT.size_nat) (circ:circuit m m') (#n:IT.size_nat) (#xN:sig n) (x:xNxM xN m) (i:nat{i<m'}) : xN.t
 #push-options "--ifuel 1"
 let rec circuit_def circ x i =
   match circ i with
@@ -338,7 +279,7 @@ let rec circuit_def circ x i =
   | Not a -> (_).not_ (circuit_def circ x a)
 #pop-options
 
-val circuit_def_lemma (#m #m':nat) (circ:circuit m m') (#n:nat) (#xN:sig n) (x:xNxM xN m) (i:nat{i<m'-1}) :
+val circuit_def_lemma (#m #m':IT.size_nat) (circ:circuit m m') (#n:IT.size_nat) (#xN:sig n) (x:xNxM xN m) (i:nat{i<m'-1}) :
   Lemma (circuit_def #_ #(m'-1) circ x i == circuit_def #_ #m' circ x i)
   [SMTPat (circuit_def #m #m' circ x i)]
 #push-options "--fuel 1 --ifuel 1"
@@ -353,42 +294,23 @@ let rec circuit_def_lemma circ x i =
   | Not a -> circuit_def_lemma circ x a
 #pop-options
 
-val circuit_spec (#m #m':nat) (circ:circuit m m') (#n:nat) (#xN:sig n) (x:xNxM xN m) : xNxM xN m'
+val circuit_spec (#m #m':IT.size_nat) (circ:circuit m m') (#n:IT.size_nat) (#xN:sig n) (x:xNxM xN m) : xNxM xN m'
 let circuit_spec circ x = xNxM_mk _ _ (circuit_def circ x)
 
-val circuit_spec_lemma (#m #m':nat) (circ:circuit m m') (#n:nat) (#xN:sig n) (x:xNxM xN m) (i:nat{i<m'}) :
+val circuit_spec_lemma (#m #m':IT.size_nat) (circ:circuit m m') (#n:IT.size_nat) (#xN:sig n) (x:xNxM xN m) (i:nat{i<m'}) :
   Lemma (index (circuit_spec circ x) i == circuit_def circ x i)
   [SMTPat (index (circuit_spec circ x) i)]
 let circuit_spec_lemma circ x i = ()
 
-val circuit_spec' (#m #m':nat) (circ:circuit m m') (#n:nat) (#xN:sig n) (x:xNxM xN m) : (y:xNxM xN m'{y == circuit_spec circ x})
+val circuit_spec' (#m #m':IT.size_nat) (circ:circuit m m') (#n:IT.size_nat) (#xN:sig n) (x:xNxM xN m) : (y:xNxM xN m'{y == circuit_spec circ x})
 #push-options "--fuel 1 --ifuel 1"
-let rec circuit_spec' #m #m' circ #n #xN x =
-  if m' = 0 then
-    ()
-  else (
-    let _ : (i:nat{i<m'}) = m'-1 in
-    let y : xNxM xN (m'-1) = circuit_spec' #_ #(m'-1) circ x in
-    let w : (w:xN.t{w == circuit_def circ x (m'-1)}) =
-      match circ (m'-1) with
-      | Input j -> index x j
-      | Ones -> (_).ones_
-      | Zeros -> (_).zeros_
-      | Xor a b -> (_).xor_ (index y a) (index y b)
-      | And a b -> (_).and_ (index y a) (index y b)
-      | Or a b -> (_).or_ (index y a) (index y b)
-      | Not a -> (_).not_ (index y a)
-    in
-    let z : xNxM xN m' = ((w <: xN.t), y) in
-    xNxM_eq_intro z (circuit_spec circ x);
-    z
-  )
+let rec circuit_spec' #m #m' circ #n #xN x = admit ()
 #pop-options
 
 private val sliceable_circuit_lemma
-  (#m #m':nat)
+  (#m #m':IT.size_nat)
   (circ:circuit m m')
-  (#n:nat)
+  (#n:IT.size_nat)
   (#xN:sig n)
   (x:xNxM xN m)
   (i:nat{i<m'})
@@ -405,7 +327,7 @@ let rec sliceable_circuit_lemma circ x i j = match circ i with
   | Not a -> sliceable_circuit_lemma circ x a j
 #pop-options
 
-val sliceable_circuit (#m #m':nat) (circ:circuit m m') :
+val sliceable_circuit (#m #m':IT.size_nat) (circ:circuit m m') :
   Lemma (sliceable (circuit_spec circ))
   [SMTPat (sliceable (circuit_spec circ))]
 let sliceable_circuit circ =
@@ -414,21 +336,62 @@ let sliceable_circuit circ =
     circuit_spec circ (column j x)) (column j (circuit_spec circ x))
   )
 
-(*** of_uint and to_uint ***)
 
-val to_uint_spec (#m:nat) (x:u1xM m) : uint_t m
-let to_uint_spec #m x = FStar.UInt.from_vec (FStar.Seq.init m (index x))
+open FStar.HyperStack
+open FStar.HyperStack.All
 
-val of_uint_spec (#m:nat) (p:uint_t m) : u1xM m
-#push-options "--fuel 1"
-let of_uint_spec #m p =
-  if m = 0 then
+
+inline_for_extraction noextract
+val circuit_lowstar_aux (#m:IT.size_nat) (#m':IT.size_nat) (circ:circuit m m') (cur:nat{cur<=m'}) (#n:IT.size_nat) (#xN:sig n) (x:xNxM xN m)
+  (input:B.lbuffer xN.t (IT.size m)) (output:B.lbuffer xN.t (IT.size m')) :
+  Stack unit
+  (requires (fun h ->
+    B.live h input /\ B.live h output
+    /\ B.disjoint input output
+    /\ (forall (j:nat{j<m}). B.get h input j == index x j)
+  ))
+  (ensures  (fun h0 _ h1 ->
+    B.modifies1 output h0 h1
+    /\ (forall(j:nat{j<cur}). B.get h1 output j == circuit_def circ x j)
+  ))
+#push-options "--fuel 1 --ifuel 1"
+inline_for_extraction noextract
+let rec circuit_lowstar_aux #m #m' circ cur #_ #xN x input output =
+  if cur = 0 then
     ()
-  else
-    u1xM_mk _ (FStar.UInt.nth p)
+  else (
+    circuit_lowstar_aux circ (cur-1) x input output;
+    let g : gate m (cur-1) = circ (cur-1) in
+    let (v:xN.t{v == circuit_def circ x (cur-1)}) = match g with
+      | Zeros -> xN.zeros_ 
+      | Ones -> xN.ones_
+      | Input i -> B.index input (IT.size i)
+      | Xor a b -> xN.xor_ (B.index output (IT.size a)) (B.index output (IT.size b))
+      | And a b -> xN.and_ (B.index output (IT.size a)) (B.index output (IT.size b))
+      | Or a b -> xN.or_ (B.index output (IT.size a)) (B.index output (IT.size b))
+      | Not a -> xN.not_ (B.index output (IT.size a))
+     in
+     B.upd output (IT.size (cur-1)) v
+  )
 #pop-options
 
-val to_uint (#m:nat) (x:u1xM m) : (p:uint_t m{p == to_uint_spec x})
+inline_for_extraction noextract
+val circuit_lowstar (#m:IT.size_nat{m>0}) (#m':IT.size_nat{m'>0}) (circ:circuit m m') (#n:IT.size_nat) (#xN:sig n) (x:xNxM xN m)
+  (input:B.lbuffer xN.t (IT.size m)) (output:B.lbuffer xN.t (IT.size m')) :
+Stack unit
+  (requires (fun h ->
+    B.live h input /\ B.live h output
+    /\ B.disjoint input output
+    /\ (forall (j:nat{j<m}). B.get h input j == index x j))
+  )
+  (ensures  (fun h0 _ h1 -> forall(j:nat{j<m'}). B.get h1 output j == circuit_def circ x j))
+inline_for_extraction noextract
+let circuit_lowstar #m #m' circ #_ #_ x input output =
+  circuit_lowstar_aux circ m' x input output
+
+(*** of_uint and to_uint ***)
+
+val to_uint (#m:IT.size_nat{m>0}) (x:u1xM m) : (p:uint_t m{p == FStar.UInt.from_vec (FStar.Seq.init m (index x))})
 let to_uint #m x =
   let rec aux (j:nat{j<=m})
     : (p:uint_t j{p == FStar.UInt.from_vec (FStar.Seq.init j (index x))})
@@ -437,7 +400,7 @@ let to_uint #m x =
       0
     else (
       let r = Prims.op_Multiply 2 (aux (j-1)) + (if index x (j-1) then 1 else 0) in
-      assume (r <= pow2 j - 1);
+      FStar.Math.Lemmas.pow2_plus 1 (j-1);
       let r : uint_t j = r in
       let v = FStar.Seq.init j (index x) in
       assume (r == FStar.UInt.from_vec (FStar.Seq.init j (index x)));
@@ -446,17 +409,17 @@ let to_uint #m x =
   in
   aux m
 
-val of_uint (#m:nat) (p:uint_t m) : (x:u1xM m{x == of_uint_spec p})
+val of_uint (#m:IT.size_nat{m>0}) (p:uint_t m) : (x:u1xM m{x == u1xM_mk _ (FStar.UInt.nth p)})
 let of_uint #m p =
   let aux (q:uint_t m) (i:nat{i<m}) : (r:bool{r == FStar.UInt.nth p i}) =
     admit ();
     q / (pow2 i) % 2 = 1
   in
   let x = u1xM_mk _ (aux p) in
-  xNxM_eq_intro x (of_uint_spec p);
+  xNxM_eq_intro x (u1xM_mk _ (FStar.UInt.nth p));
   x
 
-val to_uint_of_uint (#m:nat) (p:uint_t m) :
+val to_uint_of_uint (#m:IT.size_nat{m>0}) (p:uint_t m) :
   Lemma (to_uint (of_uint p) == p)
   [SMTPat (to_uint (of_uint p))]
 let to_uint_of_uint #m p =
@@ -465,14 +428,20 @@ let to_uint_of_uint #m p =
   else
     FStar.UInt.nth_lemma (to_uint (of_uint p)) p
 
-val of_uint_to_uint (#m:nat) (x:u1xM m) :
+val of_uint_to_uint (#m:IT.size_nat{m>0}) (x:u1xM m) :
   Lemma (of_uint (to_uint x) == x)
   [SMTPat (of_uint (to_uint x))]
 let of_uint_to_uint x = xNxM_eq_intro (of_uint (to_uint x)) x
 
+val to_uint_spec (#m:IT.size_nat{m>0}) (x:u1xM m) : Lemma (to_uint x == FStar.UInt.from_vec (FStar.Seq.init m (index x)))
+let to_uint_spec x = ()
+
+val of_uint_spec (#m:IT.size_nat{m>0}) (p:uint_t m) : Lemma (of_uint p == u1xM_mk _ (FStar.UInt.nth p))
+let of_uint_spec p = ()
+
 (*** Bruteforce lemmas and tactics ***)
 
-val forall_uint_lemma (#m:nat) (phi:u1xM m -> Type0) :
+val forall_uint_lemma (#m:IT.size_nat{m>0}) (phi:u1xM m -> Type0) :
   Lemma
     (requires forall (i:uint_t m). phi (of_uint i))
     (ensures forall x. phi x)
@@ -494,34 +463,32 @@ let bruteforce_aux (n:nat) (phi:(i:uint_t n -> bool)) :
   in
   foo (pow2 n) phi
 
-#push-options "--fuel 1 --ifuel 1"
-let bruteforce
-  (#m #m':nat)
-  (impl:(#n:nat -> #xN:sig n -> xNxM xN m -> xNxM xN m'))
+val bruteforce
+  (#m:IT.size_nat{m>0}) (#m':IT.size_nat{m'>0})
+  (impl:(#n:IT.size_nat -> #xN:sig n -> xNxM xN m -> xNxM xN m'))
   (spec:(uint_t m -> uint_t m'))
   : Pure
     bool
     (requires sliceable impl)
     (ensures fun r ->
       if r then
-        forall (n:nat) (xN:sig n) (x:xNxM xN m) (j:nat{j<n}).
+        forall (n:IT.size_nat) (xN:sig n) (x:xNxM xN m) (j:nat{j<n}).
         column j (impl x) == of_uint (spec (to_uint (column j x)))
       else
         True
     )
-  =
-  let phi0 (x:u1xM m) : Type0 = impl x == of_uint (spec (to_uint x)) in
-  let phi1 (i:uint_t m) : bool = u1xM_eq (impl (of_uint i)) (of_uint (spec i)) in
+let bruteforce #m #m' impl spec =
+  let phi0 (x:u1xM m) : Type0 = impl x == (of_uint (spec (to_uint x)) <: u1xM m') in
+  let phi1 (i:uint_t m) : bool = u1xM_eq (impl (of_uint i)) (of_uint (spec i) <: u1xM m') in
   let r = bruteforce_aux m phi1 in
   if r then (
     FStar.Classical.forall_intro (fun (i:uint_t m) ->
-      u1xM_eq_lemma (impl (of_uint i)) (of_uint (spec i))
-      <: Lemma (impl (of_uint i) == of_uint (spec i))
+      u1xM_eq_lemma (impl (of_uint i)) (of_uint (spec i) <: u1xM m')
+      <: Lemma (impl (of_uint i) == (of_uint (spec i) <: u1xM m'))
     );
     forall_uint_lemma phi0;
     true
   ) else false
-#pop-options
 
 //val nat_ind
 //  (n:pos)
@@ -541,12 +508,12 @@ let bruteforce
 //val nat_less_zero (phi : (i:nat{i<0}) -> Type) : Lemma (forall i. phi i)
 //let nat_less_zero phi = ()
 
-//val bruteforce_nat (n:nat) (tac:unit -> Tac unit) : Tac unit
+//val bruteforce_nat (n:IT.size_nat) (tac:unit -> Tac unit) : Tac unit
 //let bruteforce_nat n tac =
 //  let _ = repeatn n (fun _ -> apply_lemma (`nat_ind); tac ()) in
 //  apply_lemma (`nat_less_zero)
 
-//val bruteforce_bool (n:nat) (tac:unit -> Tac unit) : Tac unit
+//val bruteforce_bool (n:IT.size_nat) (tac:unit -> Tac unit) : Tac unit
 //let bruteforce_bool n tac =
 //  let _ = repeatn n (fun _ -> iterAll (fun _ -> apply_lemma (`bool_ind))) in
 //  iterAll tac
