code/circ/Hacl.Circuit.fst
@@ -1,0 +1,18 @@
+module Hacl.Circuit
+
+open Lib.Sliceable
+open Lib.Bitmap
+open Lib.IntTypes
+
+inline_for_extraction noextract
+let m = 1
+
+inline_for_extraction noextract
+let m' = 4
+
+inline_for_extraction noextract
+let circ : circuit 1 4 = fun (i:nat{i<4}) -> match i with
+| 0 -> Input 0
+| i -> Xor (i-1) (i-1)
+
+let impl = circuit_lowstar #m #m' circ #8 #(uN U8 PUB 8)
